src/go_lang/examples/append_log.v
@@ -10,12 +10,18 @@ From Perennial.go_lang Require Import ffi.disk_prelude.
    appends, which are implemented by atomically updating an on-disk header with
    the number of valid blocks in the log. *)
 
-(* Enc is a stateful encoder for a single disk block. *)
 Module Enc.
+  (* TODO: use this instead of encoding manually *)
   Definition S := struct.decl [
     "b" :: disk.blockT;
     "off" :: refT uint64T
   ].
+  Definition T: ty := struct.t S.
+  Definition Ptr: ty := struct.ptrT S.
+  Section fields.
+    Context `{ext_ty: ext_types}.
+    Definition get := struct.get S.
+  End fields.
 End Enc.
 
 Definition NewEnc: val :=
@@ -24,33 +30,28 @@ Definition NewEnc: val :=
       "b" ::= NewSlice byteT disk.BlockSize;
       "off" ::= ref (zero_val uint64T)
     ].
-Theorem NewEnc_t: ⊢ NewEnc : (unitT -> struct.t Enc.S).
-Proof. typecheck. Qed.
-Hint Resolve NewEnc_t : types.
 
 Definition Enc__PutInt: val :=
   λ: "enc" "x",
-    let: "off" := !(struct.get Enc.S "off" "enc") in
-    UInt64Put (SliceSkip (struct.get Enc.S "b" "enc") "off") "x";;
-    struct.get Enc.S "off" "enc" <- !(struct.get Enc.S "off" "enc") + #8.
-Theorem Enc__PutInt_t: ⊢ Enc__PutInt : (struct.t Enc.S -> uint64T -> unitT).
-Proof. typecheck. Qed.
-Hint Resolve Enc__PutInt_t : types.
+    let: "off" := !(Enc.get "off" "enc") in
+    UInt64Put (SliceSkip (Enc.get "b" "enc") "off") "x";;
+    Enc.get "off" "enc" <- !(Enc.get "off" "enc") + #8.
 
 Definition Enc__Finish: val :=
   λ: "enc",
-    struct.get Enc.S "b" "enc".
-Theorem Enc__Finish_t: ⊢ Enc__Finish : (struct.t Enc.S -> disk.blockT).
-Proof. typecheck. Qed.
-Hint Resolve Enc__Finish_t : types.
+    Enc.get "b" "enc".
 
-(* Dec is a stateful decoder that returns values encoded
-   sequentially in a single disk block. *)
 Module Dec.
   Definition S := struct.decl [
     "b" :: disk.blockT;
     "off" :: refT uint64T
   ].
+  Definition T: ty := struct.t S.
+  Definition Ptr: ty := struct.ptrT S.
+  Section fields.
+    Context `{ext_ty: ext_types}.
+    Definition get := struct.get S.
+  End fields.
 End Dec.
 
 Definition NewDec: val :=
@@ -59,42 +60,36 @@ Definition NewDec: val :=
       "b" ::= "b";
       "off" ::= ref (zero_val uint64T)
     ].
-Theorem NewDec_t: ⊢ NewDec : (disk.blockT -> struct.t Dec.S).
-Proof. typecheck. Qed.
-Hint Resolve NewDec_t : types.
 
 Definition Dec__GetInt: val :=
   λ: "dec",
-    let: "off" := !(struct.get Dec.S "off" "dec") in
-    struct.get Dec.S "off" "dec" <- !(struct.get Dec.S "off" "dec") + #8;;
-    UInt64Get (SliceSkip (struct.get Dec.S "b" "dec") "off").
-Theorem Dec__GetInt_t: ⊢ Dec__GetInt : (struct.t Dec.S -> uint64T).
-Proof. typecheck. Qed.
-Hint Resolve Dec__GetInt_t : types.
+    let: "off" := !(Dec.get "off" "dec") in
+    Dec.get "off" "dec" <- !(Dec.get "off" "dec") + #8;;
+    UInt64Get (SliceSkip (Dec.get "b" "dec") "off").
 
 Module Log.
   Definition S := struct.decl [
     "sz" :: uint64T;
     "diskSz" :: uint64T
   ].
+  Definition T: ty := struct.t S.
+  Definition Ptr: ty := struct.ptrT S.
+  Section fields.
+    Context `{ext_ty: ext_types}.
+    Definition get := struct.get S.
+  End fields.
 End Log.
 
 Definition Log__mkHdr: val :=
   λ: "log",
     let: "enc" := NewEnc #() in
-    Enc__PutInt "enc" (struct.get Log.S "sz" "log");;
-    Enc__PutInt "enc" (struct.get Log.S "diskSz" "log");;
+    Enc__PutInt "enc" (Log.get "sz" "log");;
+    Enc__PutInt "enc" (Log.get "diskSz" "log");;
     Enc__Finish "enc".
-Theorem Log__mkHdr_t: ⊢ Log__mkHdr : (struct.t Log.S -> disk.blockT).
-Proof. typecheck. Qed.
-Hint Resolve Log__mkHdr_t : types.
 
 Definition Log__writeHdr: val :=
   λ: "log",
     disk.Write #0 (Log__mkHdr "log").
-Theorem Log__writeHdr_t: ⊢ Log__writeHdr : (struct.t Log.S -> unitT).
-Proof. typecheck. Qed.
-Hint Resolve Log__writeHdr_t : types.
 
 Definition Init: val :=
   λ: "diskSz",
@@ -111,9 +106,6 @@ Definition Init: val :=
       ] in
       Log__writeHdr "log";;
       ("log", #true)).
-Theorem Init_t: ⊢ Init : (uint64T -> (struct.t Log.S * boolT)).
-Proof. typecheck. Qed.
-Hint Resolve Init_t : types.
 
 Definition Open: val :=
   λ: <>,
@@ -125,27 +117,18 @@ Definition Open: val :=
       "sz" ::= "sz";
       "diskSz" ::= "diskSz"
     ].
-Theorem Open_t: ⊢ Open : (unitT -> struct.t Log.S).
-Proof. typecheck. Qed.
-Hint Resolve Open_t : types.
 
 Definition Log__Get: val :=
   λ: "log" "i",
-    let: "sz" := struct.get Log.S "sz" "log" in
+    let: "sz" := Log.get "sz" "log" in
     (if: "i" < "sz"
     then (disk.Read (#1 + "i"), #true)
     else (slice.nil, #false)).
-Theorem Log__Get_t: ⊢ Log__Get : (struct.t Log.S -> uint64T -> (disk.blockT * boolT)).
-Proof. typecheck. Qed.
-Hint Resolve Log__Get_t : types.
 
 Definition writeAll: val :=
   λ: "bks" "off",
     ForSlice "i" "bk" "bks"
       (disk.Write ("off" + "i") "bk").
-Theorem writeAll_t: ⊢ writeAll : (slice.T disk.blockT -> uint64T -> unitT).
-Proof. typecheck. Qed.
-Hint Resolve writeAll_t : types.
 
 Definition Log__Append: val :=
   λ: "log" "bks",
@@ -161,9 +144,6 @@ Definition Log__Append: val :=
       Log__writeHdr "newLog";;
       struct.store Log.S "log" "newLog";;
       #true).
-Theorem Log__Append_t: ⊢ Log__Append : (struct.ptrT Log.S -> slice.T disk.blockT -> boolT).
-Proof. typecheck. Qed.
-Hint Resolve Log__Append_t : types.
 
 Definition Log__Reset: val :=
   λ: "log",
@@ -173,6 +153,3 @@ Definition Log__Reset: val :=
     ] in
     Log__writeHdr "newLog";;
     struct.store Log.S "log" "newLog".
-Theorem Log__Reset_t: ⊢ Log__Reset : (struct.ptrT Log.S -> unitT).
-Proof. typecheck. Qed.
-Hint Resolve Log__Reset_t : types.
